\left(
 \begin{matrix}n\\k\end{matrix}
\right)
=
\left(
 \begin{matrix}n-1\\k-1\end{matrix}
\right)
+
\left(
 \begin{matrix}n\\k-1\end{matrix}
\right)

\frac{\left(n-1\right)! \cdot k+\left(n-1\right)! \cdot \left(n-k\right) 
}{\left(n-k\right)!\cdot \left(k-1\right)!\cdot k}=\frac{\left(n-1\right)! \cdot \left(k+n-k\right)}{\left(n-k\right)!\cdot k!}=\frac{n!}{\left(n-k\right)!\cdot k!}
\\
\\
+\frac{\left(n-1\right)! \cdot \left(n-k\right)}{\left(n-k-1\right)!\cdot k! \cdot \left(n-k\right)} \; (2)
\\
\\
\left(\begin{matrix}n\\k\end{matrix}\right)=\left(\begin{matrix}n-1\\k-1\end{matrix}\right)+\left(\begin{matrix}n\\k-1\end{matrix}\right) = C_{k}^{n} = C_{k-1}^{n-1} + C_{k-1}^{n}
